theories/lithium/interpreter.v
@@ -28,16 +28,6 @@ Section coq_tactics.
     (P1 -∗ P2) → envs_entails Δ (P1 ∗ T) → envs_entails Δ (P2 ∗ T).
   Proof. by rewrite envs_entails_eq => -> HP. Qed.
 
-  Lemma tac_vm_compute_hint {A B} Δ (f : A → option B) a (Q : B → iProp Σ) x:
-    (∀ y, Some x = y → f a = y) →
-    envs_entails Δ (Q x) →
-    envs_entails Δ (vm_compute_hint f a Q).
-  Proof.
-    rewrite envs_entails_eq. intros ? HQ.
-    etrans; [done|]. etrans; [ |apply: bi.exist_intro].
-    iIntros "$ !%". naive_solver.
-  Qed.
-
   Lemma tac_protected_eq_app {A} (f : A → Prop) a :
     f a → f (protected a).
   Proof. by rewrite protected_eq. Qed.
@@ -689,11 +679,11 @@ Ltac liDestructHint :=
     end
   end; repeat (liForall || liImpl); try by [exfalso; can_solve_tac].
 
-Ltac liVmComputeHint :=
+Ltac liTacticHint :=
   lazymatch goal with
-  | |- envs_entails ?Δ (vm_compute_hint ?f ?a _) =>
-      refine (tac_vm_compute_hint _ _ _ _ _ _ _);
-        [let H := fresh in intros ? H; vm_compute; apply H|]
+  | |- envs_entails ?Δ (tactic_hint ?t ?T) =>
+      let x := constr:(_ : TacticHint t) in
+      refine (tac_fast_apply (x.(tactic_hint_proof) T) _)
   end.
 
 Ltac liAccu :=
@@ -792,7 +782,7 @@ Ltac liStep :=
     | liSideCond
     | liFindInContext
     | liDestructHint
-    | liVmComputeHint
+    | liTacticHint
     | liTrue
     | liFalse
     | liAccu
